Use lexsort and hdsort

theories/BWT/BurrowsWheeler.v
@@ -18,7 +18,8 @@ Require Import BWT.Lib.Repeat.
 Require Import BWT.Rotation.Rotation.
 Require Import BWT.Rotation.Rots.
 Require Import BWT.Sorting.Ord.
-Require Import BWT.Sorting.Prefix.
+Require Import BWT.Sorting.Lexicographic.
+Require Import BWT.Sorting.Key.
 
 Import Coq.Lists.List.ListNotations.
 
@@ -28,12 +29,12 @@ Section Transform.
   Definition bwp (l: list A) : list A :=
     match l with
     | [] => []
-    | hd :: tl => List.map (fun x => last x hd) (sort (length l) (rots l))
+    | hd :: tl => List.map (fun x => last x hd) (lexsort (rots l))
     end.
 
   Lemma bwp_nonempty : forall l d,
       l <> [] ->
-      bwp l = List.map (fun x => last x d) (sort (length l) (rots l)).
+      bwp l = List.map (fun x => last x d) (lexsort (rots l)).
   Proof.
     destruct l; intros.
     - contradiction.
@@ -41,8 +42,8 @@ Section Transform.
       apply Forall_forall.
       intros x HIn.
       assert (x <> []). {
-        apply (Forall_forall (fun x => ~ x = []) (sort (length (a :: l)) (rots (a :: l)))); auto.
-        eapply Permutation_forall. apply sort_perm.
+        apply (Forall_forall (fun x => ~ x = []) (lexsort (rots (a :: l)))); auto.
+        eapply Permutation_forall. apply lexsort_perm.
         apply rots_nonempty; auto.
       }
       apply last_nonempty; auto.
@@ -54,25 +55,25 @@ Section Transform.
     induction l.
     - reflexivity.
     - simpl. rewrite map_length.
-      rewrite sort_length.
+      rewrite lexsort_length.
       rewrite rots_length.
       reflexivity.
   Qed.
 
   Definition bwn (l : list A) : nat :=
-    findIndex l (sort (length l) (rots l)).
+    findIndex l (lexsort (rots l)).
 
-  Lemma orig_in_sorted_rots : forall l k,
-      l <> [] -> Exists (eq l) (sort k (rots l)).
+  Lemma orig_in_sorted_rots : forall l,
+      l <> [] -> Exists (eq l) (lexsort (rots l)).
   Proof.
     intros.
-    apply Permutation_exists with (l0 := rots l) (l' := sort k (rots l)).
-    apply sort_perm.
+    apply Permutation_exists with (l0 := rots l) (l' := lexsort (rots l)).
+    apply lexsort_perm.
     apply orig_in_rots. auto.
   Qed.
 
   Theorem bwn_correct : forall xs d,
-    xs <> [] -> nth (bwn xs) (sort (length xs) (rots xs)) d = xs.
+    xs <> [] -> nth (bwn xs) (lexsort (rots xs)) d = xs.
   Proof.
     intros.
     unfold bwn.
@@ -87,19 +88,19 @@ Section Recreate.
   Fixpoint recreate (j : nat) (l : list A) : list (list A) :=
     match j with
     | O    => map (const []) l
-    | S j' => sort 1 (prepend_col l (recreate j' l))
+    | S j' => hdsort (prepend_col l (recreate j' l))
     end.
 
   Theorem recreate_correct_ind : forall j l,
       j <= length l ->
-      recreate j (bwp l) = cols j (sort (length l) (rots l)).
+      recreate j (bwp l) = cols j (lexsort (rots l)).
   Proof.
     induction j as [|j IH]; intros l HJ.
     - unfold cols; simpl.
       do 2 (erewrite map_const; [|unfold const; reflexivity]).
-      rewrite bwp_length, sort_length, rots_length.
+      rewrite bwp_length, lexsort_length, rots_length.
       reflexivity.
-    - rewrite <- sort_rots_hdsort.
+    - rewrite <- lexsort_rots_hdsort.
       rewrite cols_S_hdsort.
       destruct (length_nonempty_destr l j) as [HNE d]; [auto|].
       rewrite cols_rrot with (d0 := d).
@@ -108,16 +109,16 @@ Section Recreate.
       reflexivity.
   Qed.
 
-  Lemma sort_rots_len : forall k l,
-      Forall (fun x => length x = length l) (sort k (rots l)).
+  Lemma sort_rots_len : forall l,
+      Forall (fun x => length x = length l) (lexsort (rots l)).
   Proof.
     intros.
     eapply Permutation_forall.
-    apply sort_perm. apply rots_row_length.
+    apply lexsort_perm. apply rots_row_length.
   Qed.
 
   Corollary recreate_correct : forall l,
-      recreate (length l) (bwp l) = sort (length l) (rots l).
+      recreate (length l) (bwp l) = lexsort (rots l).
   Proof.
     intros.
     rewrite recreate_correct_ind by omega.
