theories/BWT/Instances.v
@@ -1,5 +1,6 @@
 Require compcert.lib.Integers.
 Require Import Coq.ZArith.ZArith.
+Require Import Ascii.
 Require Export Coq.Classes.EquivDec.
 
 Require Export BWT.Sorting.Ord.
@@ -10,6 +11,8 @@ Instance Int64_EqDec  : EqDec Integers.Int64.int  eq := Integers.Int64.eq_dec.
 Instance Ptrofs_EqDec : EqDec Integers.Ptrofs.int eq := Integers.Ptrofs.eq_dec.
 
 Instance EqDec_Z : EqDec Z eq := BinInt.Z.eq_dec.
+
+Instance EqDec_ascii : EqDec ascii eq := ascii_dec.
 
 Instance Ord_nat : Ord nat :=
   { le := Nat.le;
@@ -42,3 +45,11 @@ Instance Int64_Ord : Ord Integers.Int64.int :=
   int_Ord Integers.Int64.repr_unsigned.
 Instance Ptrofs_Ord : Ord Integers.Ptrofs.int :=
   int_Ord Integers.Ptrofs.repr_unsigned.
+
+Instance Ascii_Ord : Ord ascii.
+Proof.
+  apply Build_Ord with (le := (fun x y => le (nat_of_ascii x) (nat_of_ascii y))).
+  - intros x y z; exact (le_trans (nat_of_ascii x) (nat_of_ascii y) (nat_of_ascii z)).
+  - intros; exact (le_total (nat_of_ascii x) (nat_of_ascii y)).
+  - intros; exact (le_dec (nat_of_ascii x) (nat_of_ascii y)).
+Defined.
