theories/BWT/Sorting/Key.v
@@ -1,0 +1,23 @@
+Require Import Coq.Lists.List.
+
+Require Import BWT.Sorting.Ord.
+Require Import BWT.Sorting.Mergesort.
+Require Import BWT.Sorting.Lexicographic.
+
+Section KeyOrd.
+  Context {K : Type} `{O: Ord K}.
+
+  Definition keyOrd {A : Type} (key : A -> K) : Ord A.
+  Proof.
+    apply Build_Ord with (le := fun x y => le (key x) (key y));
+      intros; eauto using le_trans, le_total, le_dec.
+  Defined.
+End KeyOrd.
+
+Section HdSort.
+  Context {A : Type} `{O: Ord A}.
+
+  Program Definition hdsort : list (list A) -> list (list A)
+    := @mergesort _ (keyOrd (firstn 1)).
+
+End HdSort.
