theories/BWT/Sorting/Lexicographic.v
@@ -1,0 +1,104 @@
+(** An implementation of equivalence and lexicographic ordering for
+    lists, only looking at the first k elements of the list. **)
+
+Require Import Coq.Lists.List.
+Require Import Coq.omega.Omega.
+Require Import Coq.Relations.Relation_Definitions.
+Require Import Coq.Classes.EquivDec.
+Require Import Coq.Sorting.Permutation.
+
+Require Import BWT.Sorting.Ord.
+Require Import BWT.Sorting.Mergesort.
+
+Import Coq.Lists.List.ListNotations.
+
+Section LexLe.
+  Context {A : Type} `{O: Ord A}.
+
+  Inductive lex_le : list A -> list A -> Prop :=
+  | lex_le_nil : forall ys, lex_le [] ys
+  | le_cons_lt : forall x y xs ys, lt x y -> lex_le (x :: xs) (y :: ys)
+  | le_cons_eq : forall x y xs ys, eqv x y -> lex_le xs ys ->
+                              lex_le (x :: xs) (y :: ys).
+
+  Theorem lex_le_trans : forall x y z, lex_le x y -> lex_le y z -> lex_le x z.
+  Proof.
+    intros x y z LXY. revert z.
+    induction LXY as [|x y xs ys HLT|x y xs ys HE HLex IH]; intros z LYZ;
+      [constructor|inversion LYZ; subst; clear LYZ..];
+      rename y0 into z; rename ys0 into zs.
+    - apply le_cons_lt. eapply lt_trans; eauto.
+    - apply le_cons_lt. rewrite <- H1. auto.
+    - apply le_cons_lt. rewrite HE. auto.
+    - apply le_cons_eq.
+      eapply eqv_trans; eauto.
+      apply IH; auto.
+  Defined.
+
+  Theorem lex_le_total : forall x y, lex_le x y \/ lex_le y x.
+  Proof.
+    induction x as [|x xs]; [left; constructor|].
+    intros [|y ys]; [right; constructor|].
+    destruct (lt_eq_dec x y) as [[LXY|E]|LYX]; eauto using le_cons_lt.
+    edestruct IHxs; eauto using le_cons_eq, eqv_sym.
+  Defined.
+
+  Program Fixpoint lex_le_dec xs ys : { lex_le xs ys } + { ~ lex_le xs ys } :=
+    match (xs, ys) with
+    | (nil, _)      => left  _
+    | (_ :: _, nil) => right _
+    | (x :: xs, y :: ys) =>
+      match lt_eq_dec x y with
+      | inleft (left _) => left _  (* < *)
+      | inright _       => right _ (* > *)
+      | inleft (right _) =>
+        match (lex_le_dec xs ys) with
+        | left  _ => left _
+        | right _ => right _
+        end
+      end
+    end.
+  Next Obligation. constructor. Defined.
+  Next Obligation. intro c; inversion c. Defined.
+  Next Obligation. apply le_cons_lt. auto. Defined.
+  Next Obligation.
+    intro c. inversion c; subst; clear c.
+    - eapply lt_excl; split; eauto.
+    - eapply lt_not_eq; eauto using eqv_sym.
+  Defined.
+  Next Obligation. apply le_cons_eq; auto. Defined.
+  Next Obligation.
+    intro c. inversion c; subst; clear c.
+    - eapply lt_not_eq; eauto.
+    - contradiction.
+  Defined.
+End LexLe.
+
+Instance Ord_list_lex {A} `{Ord A} : Ord (list A) :=
+  { le := lex_le;
+    le_trans := lex_le_trans;
+    le_total := lex_le_total;
+    le_dec := lex_le_dec;
+  }.
+
+Section LexSort.
+  Context {A : Type} `{Ord A}.
+
+  Definition lexsort : list (list A) -> list (list A)
+    := fun l => proj1_sig (@mergesort _ Ord_list_lex l).
+
+  Theorem lexsort_perm : forall l, Permutation l (lexsort l).
+  Proof.
+    intros.
+    unfold lexsort. case (mergesort l). intros l' [S [P St]].
+    cbn. apply Permutation_sym. apply P.
+  Defined.
+
+  Theorem lexsort_length : forall l,
+      length (lexsort l) = length l.
+  Proof.
+    intros.
+    apply Permutation_length.
+    apply Permutation_sym. apply lexsort_perm.
+  Qed.
+End LexSort.
